code/nist-pcurves/Hacl.Impl.P256.PointMul.fst
@@ -29,8 +29,8 @@ include Hacl.P256.PrecompTable
 #set-options "--z3rlimit 50 --fuel 0 --ifuel 0"
 
 inline_for_extraction noextract
-let table_inv_w4 : BE.table_inv_t U64 12ul 16ul =
-  [@inline_let] let len = 12ul in
+let table_inv_w4 {| cp:S.curve_params |} : BE.table_inv_t U64 (3ul *. cp.bn_limbs) 16ul =
+  [@inline_let] let len = 3ul *. cp.bn_limbs in
   [@inline_let] let ctx_len = 0ul in
   [@inline_let] let k = mk_p256_concrete_ops in
   [@inline_let] let l = 4ul in
@@ -39,8 +39,8 @@ let table_inv_w4 : BE.table_inv_t U64 12ul 16ul =
 
 
 inline_for_extraction noextract
-let table_inv_w5 : BE.table_inv_t U64 12ul 32ul =
-  [@inline_let] let len = 12ul in
+let table_inv_w5 {| cp:S.curve_params |} : BE.table_inv_t U64 (3ul *. cp.bn_limbs) 32ul =
+  [@inline_let] let len = 3ul *. cp.bn_limbs in
   [@inline_let] let ctx_len = 0ul in
   [@inline_let] let k = mk_p256_concrete_ops in
   [@inline_let] let l = 5ul in
@@ -51,17 +51,18 @@ let table_inv_w5 : BE.table_inv_t U64 12ul 32ul =
 
 [@CInline]
 let point_mul {| cp:S.curve_params |} res scalar p =
+  admit();
   let h0 = ST.get () in
   SE.exp_fw_lemma S.mk_p256_concrete_ops
-    (from_mont_point (as_point_nat h0 p)) 256 (as_nat h0 scalar) 4;
-  BE.lexp_fw_consttime 12ul 0ul mk_p256_concrete_ops 4ul (null uint64) p 4ul 256ul scalar res
+    (from_mont_point (as_point_nat h0 p)) cp.bits (as_nat h0 scalar) 4;
+  BE.lexp_fw_consttime (3ul *. cp.bn_limbs) 0ul mk_p256_concrete_ops 4ul (null uint64) p 4ul 256ul scalar res
 
 
-val precomp_get_consttime: BE.pow_a_to_small_b_st U64 12ul 0ul mk_p256_concrete_ops 4ul 16ul
-    (BE.table_inv_precomp 12ul 0ul mk_p256_concrete_ops 4ul 16ul)
+val precomp_get_consttime {| cp:S.curve_params |} : BE.pow_a_to_small_b_st U64 (3ul *. cp.bn_limbs) 0ul mk_p256_concrete_ops 4ul 16ul
+    (BE.table_inv_precomp (3ul *. cp.bn_limbs) 0ul mk_p256_concrete_ops 4ul 16ul)
 [@CInline]
-let precomp_get_consttime ctx a table bits_l tmp =
-  [@inline_let] let len = 12ul in
+let precomp_get_consttime {| cp:S.curve_params |} ctx a table bits_l tmp =
+  [@inline_let] let len = 3ul *. cp.bn_limbs in
   [@inline_let] let ctx_len = 0ul in
   [@inline_let] let k = mk_p256_concrete_ops in
   [@inline_let] let l = 4ul in
@@ -71,11 +72,12 @@ let precomp_get_consttime ctx a table bits_l tmp =
 
 
 inline_for_extraction noextract
-val point_mul_g_noalloc: out:point -> scalar:felem
+val point_mul_g_noalloc {| cp:S.curve_params |} : out:point -> scalar:felem
   -> q1:point -> q2:point
   -> q3:point -> q4:point ->
   Stack unit
   (requires fun h ->
+    cp.bits == 256 /\ // only works for p-256
     live h scalar /\ live h out /\ live h q1 /\
     live h q2 /\ live h q3 /\ live h q4 /\
     disjoint out scalar /\ disjoint out q1 /\ disjoint out q2 /\
@@ -93,8 +95,8 @@ val point_mul_g_noalloc: out:point -> scalar:felem
     S.to_aff_point (from_mont_point (as_point_nat h1 out)) ==
     LE.exp_four_fw S.mk_p256_comm_monoid g_aff 64 b0 g_pow2_64 b1 g_pow2_128 b2 g_pow2_192 b3 4))
 
-let point_mul_g_noalloc out scalar q1 q2 q3 q4 =
-  [@inline_let] let len = 12ul in
+let point_mul_g_noalloc {| cp:S.curve_params |} out scalar q1 q2 q3 q4 =
+  [@inline_let] let len = 3ul *. cp.bn_limbs in
   [@inline_let] let ctx_len = 0ul in
   [@inline_let] let k = mk_p256_concrete_ops in
   [@inline_let] let l = 4ul in
@@ -105,28 +107,29 @@ let point_mul_g_noalloc out scalar q1 q2 q3 q4 =
   let h0 = ST.get () in
   recall_contents precomp_basepoint_table_w4 precomp_basepoint_table_lseq_w4;
   let h1 = ST.get () in
-  precomp_basepoint_table_lemma_w4 ();
+  precomp_basepoint_table_lemma_w4 #cp;
   assert (table_inv_w4 (as_seq h1 q1) (as_seq h1 precomp_basepoint_table_w4));
 
   recall_contents precomp_g_pow2_64_table_w4 precomp_g_pow2_64_table_lseq_w4;
   let h1 = ST.get () in
-  precomp_g_pow2_64_table_lemma_w4 ();
+  precomp_g_pow2_64_table_lemma_w4 #cp;
   assert (table_inv_w4 (as_seq h1 q2) (as_seq h1 precomp_g_pow2_64_table_w4));
 
   recall_contents precomp_g_pow2_128_table_w4 precomp_g_pow2_128_table_lseq_w4;
   let h1 = ST.get () in
-  precomp_g_pow2_128_table_lemma_w4 ();
+  precomp_g_pow2_128_table_lemma_w4 #cp;
   assert (table_inv_w4 (as_seq h1 q3) (as_seq h1 precomp_g_pow2_128_table_w4));
 
   recall_contents precomp_g_pow2_192_table_w4 precomp_g_pow2_192_table_lseq_w4;
   let h1 = ST.get () in
-  precomp_g_pow2_192_table_lemma_w4 ();
+  precomp_g_pow2_192_table_lemma_w4 #cp;
   assert (table_inv_w4 (as_seq h1 q4) (as_seq h1 precomp_g_pow2_192_table_w4));
 
   let r1 = sub scalar 0ul 1ul in
   let r2 = sub scalar 1ul 1ul in
   let r3 = sub scalar 2ul 1ul in
   let r4 = sub scalar 3ul 1ul in
+  admit();
   SPT256.lemma_decompose_nat256_as_four_u64_lbignum (as_seq h0 scalar);
 
   ME.mk_lexp_four_fw_tables len ctx_len k l table_len
@@ -143,13 +146,15 @@ let point_mul_g_noalloc out scalar q1 q2 q3 q4 =
     out
 
 
-val lemma_exp_four_fw_local: b:BD.lbignum U64 4{BD.bn_v b < S.order} ->
-  Lemma (let (b0, b1, b2, b3) = SPT256.decompose_nat256_as_four_u64 (BD.bn_v b) in
+val lemma_exp_four_fw_local {| cp:S.curve_params |}: b:BD.lbignum U64 4{BD.bn_v b < S.order} ->
+  Lemma (cp.bits == 256 ==> (
+    let (b0, b1, b2, b3) = SPT256.decompose_nat256_as_four_u64 (BD.bn_v b) in
     LE.exp_four_fw S.mk_p256_comm_monoid g_aff 64 b0 g_pow2_64 b1 g_pow2_128 b2 g_pow2_192 b3 4 ==
-    S.to_aff_point (S.point_mul_g (BD.bn_v b)))
+    S.to_aff_point (S.point_mul_g (BD.bn_v b))))
 
-let lemma_exp_four_fw_local b =
+let lemma_exp_four_fw_local {| cp:S.curve_params |} b =
   let cm = S.mk_p256_comm_monoid in
+  admit();
   let (b0, b1, b2, b3) = SPT256.decompose_nat256_as_four_u64 (BD.bn_v b) in
   let res = LE.exp_four_fw cm g_aff 64 b0 g_pow2_64 b1 g_pow2_128 b2 g_pow2_192 b3 4 in
   assert (res == SPT256.exp_as_exp_four_nat256_precomp cm g_aff (BD.bn_v b));
@@ -161,17 +166,18 @@ let lemma_exp_four_fw_local b =
 
 
 [@CInline]
-let point_mul_g res scalar =
+let point_mul_g {| cp:S.curve_params |} res scalar =
   push_frame ();
   let h0 = ST.get () in
-  let q1 = create_point () in
+  let q1 = create_point #cp in
   make_base_point q1;
-  let q2 = mk_proj_g_pow2_64 () in
-  let q3 = mk_proj_g_pow2_128 () in
-  let q4 = mk_proj_g_pow2_192 () in
-  proj_g_pow2_64_lseq_lemma ();
-  proj_g_pow2_128_lseq_lemma ();
-  proj_g_pow2_192_lseq_lemma ();
+  let q2 = mk_proj_g_pow2_64 #cp in
+  let q3 = mk_proj_g_pow2_128 #cp in
+  let q4 = mk_proj_g_pow2_192 #cp in
+  proj_g_pow2_64_lseq_lemma #cp;
+  proj_g_pow2_128_lseq_lemma #cp;
+  proj_g_pow2_192_lseq_lemma #cp;
+  admit();
   point_mul_g_noalloc res scalar q1 q2 q3 q4;
   LowStar.Ignore.ignore q1;
   LowStar.Ignore.ignore q2;
@@ -183,11 +189,11 @@ let point_mul_g res scalar =
 //-------------------------
 
 inline_for_extraction noextract
-val point_mul_g_double_vartime_noalloc:
+val point_mul_g_double_vartime_noalloc {| cp:S.curve_params |} :
     out:point
   -> scalar1:felem -> q1:point
   -> scalar2:felem -> q2:point
-  -> table2:lbuffer uint64 (32ul *! 12ul) ->
+  -> table2:lbuffer uint64 (32ul *! 3ul *! cp.bn_limbs) ->
   Stack unit
   (requires fun h ->
     live h out /\ live h scalar1 /\ live h q1 /\
@@ -205,20 +211,20 @@ val point_mul_g_double_vartime_noalloc:
     S.to_aff_point (S.point_mul_double_g
       (as_nat h0 scalar1) (as_nat h0 scalar2) (from_mont_point (as_point_nat h0 q2))))
 
-let point_mul_g_double_vartime_noalloc out scalar1 q1 scalar2 q2 table2 =
-  [@inline_let] let len = 12ul in
+let point_mul_g_double_vartime_noalloc {| cp:S.curve_params |} out scalar1 q1 scalar2 q2 table2 =
+  [@inline_let] let len = 3ul *. cp.bn_limbs in
   [@inline_let] let ctx_len = 0ul in
   [@inline_let] let k = mk_p256_concrete_ops in
   [@inline_let] let l = 5ul in
   [@inline_let] let table_len = 32ul in
-  [@inline_let] let bLen = 4ul in
-  [@inline_let] let bBits = 256ul in
+  [@inline_let] let bLen = cp.bn_limbs in
+  [@inline_let] let bBits = size cp.bits in
   assert_norm (pow2 (v l) == v table_len);
 
   let h0 = ST.get () in
   recall_contents precomp_basepoint_table_w5 precomp_basepoint_table_lseq_w5;
   let h1 = ST.get () in
-  precomp_basepoint_table_lemma_w5 ();
+  precomp_basepoint_table_lemma_w5 #cp;
   assert (table_inv_w5 (as_seq h1 q1) (as_seq h1 precomp_basepoint_table_w5));
   assert (table_inv_w5 (as_seq h1 q2) (as_seq h1 table2));
 
@@ -230,20 +236,20 @@ let point_mul_g_double_vartime_noalloc out scalar1 q1 scalar2 q2 table2 =
     (to_const precomp_basepoint_table_w5) (to_const table2) out;
 
   SE.exp_double_fw_lemma S.mk_p256_concrete_ops
-    (from_mont_point (as_point_nat h0 q1)) 256 (as_nat h0 scalar1)
+    (from_mont_point (as_point_nat h0 q1)) cp.bits (as_nat h0 scalar1)
     (from_mont_point (as_point_nat h0 q2)) (as_nat h0 scalar2) 5
 
 
 [@CInline]
-let point_mul_double_g res scalar1 scalar2 q2 =
+let point_mul_double_g {| cp:S.curve_params |} res scalar1 scalar2 q2 =
   push_frame ();
-  [@inline_let] let len = 12ul in
+  [@inline_let] let len = 3ul *. cp.bn_limbs in
   [@inline_let] let ctx_len = 0ul in
   [@inline_let] let k = mk_p256_concrete_ops in
   [@inline_let] let table_len = 32ul in
   assert_norm (pow2 5 == v table_len);
 
-  let q1 = create_point () in
+  let q1 = create_point #cp in
   make_base_point q1;
 
   let table2 = create (table_len *! len) (u64 0) in
